Foundation/Propositional/Kripke/Filteration.lean
@@ -1,0 +1,254 @@
+import Mathlib.Data.Set.Finite.Powerset
+import Foundation.Propositional.Kripke.Basic
+
+universe u v
+
+namespace LO.Propositional
+
+namespace Kripke
+
+open Formula (atom)
+open Formula.Kripke
+
+def filterEquiv (M : Kripke.Model) (T : FormulaSet ℕ) [T.SubformulaClosed] (x y : M.World) := ∀ φ, (_ : φ ∈ T := by trivial) → x ⊧ φ ↔ y ⊧ φ
+
+variable (M : Kripke.Model) (T : FormulaSet ℕ) [T.SubformulaClosed]
+
+lemma filterEquiv.equivalence : Equivalence (filterEquiv M T) where
+  refl := by intro x φ _; rfl;
+  symm := by intro x y h φ hp; exact h _ hp |>.symm;
+  trans := by
+    intro x y z exy eyz;
+    intro φ hp;
+    exact Iff.trans (exy φ hp) (eyz φ hp)
+
+def FilterEqvSetoid : Setoid (M.World) := ⟨filterEquiv M T, filterEquiv.equivalence M T⟩
+
+abbrev FilterEqvQuotient := Quotient (FilterEqvSetoid M T)
+
+lemma FilterEqvQuotient.finite (T_finite : T.Finite) : Finite (FilterEqvQuotient M T) := by
+  have : Finite (𝒫 T) := Set.Finite.powerset T_finite
+  let f : FilterEqvQuotient M T → 𝒫 T :=
+    λ (Qx : FilterEqvQuotient M T) => Quotient.lift (λ x => ⟨{ φ ∈ T | x ⊧ φ }, (by simp_all)⟩) (by
+      intro x y hxy;
+      suffices {φ | φ ∈ T ∧ Satisfies M x φ} = {φ | φ ∈ T ∧ Satisfies M y φ} by simpa;
+      apply Set.eq_of_subset_of_subset;
+      . rintro φ ⟨hp, hx⟩; exact ⟨hp, (hxy φ hp).mp hx⟩;
+      . rintro φ ⟨hp, hy⟩; exact ⟨hp, (hxy φ hp).mpr hy⟩;
+    ) Qx
+  have hf : Function.Injective f := by
+    intro Qx Qy h;
+    obtain ⟨x, rfl⟩ := Quotient.exists_rep Qx;
+    obtain ⟨y, rfl⟩ := Quotient.exists_rep Qy;
+    simp [f] at h;
+    apply Quotient.eq''.mpr;
+    intro φ hp;
+    constructor;
+    . intro hpx;
+      have : ∀ a ∈ T, x ⊧ a → a ∈ T ∧ y ⊧ a := by simpa using h.subset;
+      exact this φ hp hpx |>.2;
+    . intro hpy;
+      have := h.symm.subset;
+      simp only [Set.setOf_subset_setOf, and_imp, f] at this;
+      exact this φ hp hpy |>.2;
+  exact Finite.of_injective f hf
+
+instance : Nonempty (FilterEqvQuotient M T) := ⟨⟦M.toFrame.world_nonempty.some⟧⟩
+
+class FilterOf (FM : Model) (M : Model) (T : FormulaSet ℕ) [T.SubformulaClosed] : Prop where
+  def_world : FM.World = FilterEqvQuotient M T := by rfl
+  def_rel_forth : ∀ {x y : M.World}, x ≺ y → (cast def_world.symm ⟦x⟧) ≺ (cast def_world.symm ⟦y⟧)
+  def_rel_back : ∀ {Qx Qy : FM.World}, Qx ≺ Qy → Quotient.lift₂ (λ x y => ∀ φ ∈ T, (x ⊧ φ → y ⊧ φ)) (by
+    intro x₁ y₁ x₂ y₂ hx hy;
+    apply eq_iff_iff.mpr;
+    constructor;
+    . intro h φ hφ hφ_x₂;
+      apply hy φ |>.mp;
+      apply h;
+      . exact hφ
+      . apply hx φ |>.mpr hφ_x₂;
+    . intro h φ hφ hφ_y₁;
+      apply hy φ |>.mpr;
+      apply h;
+      . exact hφ
+      . apply hx φ |>.mp hφ_y₁;
+  ) (cast def_world Qx) (cast def_world Qy)
+  def_valuation Qx a : (ha : (atom a) ∈ T := by trivial) →
+    FM Qx a ↔ Quotient.lift (λ x => M x a) (by
+      intro x y h;
+      apply eq_iff_iff.mpr;
+      constructor;
+      . intro hx; exact h (.atom a) ha |>.mp hx;
+      . intro hy; exact h (.atom a) ha |>.mpr hy;
+    ) (cast def_world Qx)
+
+attribute [simp] FilterOf.def_world
+
+
+section
+
+variable {M T}
+
+lemma reflexive_filterOf_of_reflexive (h_filter : FilterOf FM M T) (hRefl : Reflexive M.toFrame) : Reflexive FM.Rel := by
+  intro Qx;
+  obtain ⟨x, hx⟩ := Quotient.exists_rep (cast (h_filter.def_world) Qx);
+  convert h_filter.def_rel_forth $ hRefl x <;> simp_all;
+
+lemma serial_filterOf_of_serial (h_filter : FilterOf FM M T) (hSerial : Serial M.toFrame) : Serial FM.Rel := by
+  intro Qx;
+  obtain ⟨x, hx⟩ := Quotient.exists_rep (cast (h_filter.def_world) Qx);
+  obtain ⟨y, Rxy⟩ := hSerial x;
+  use (cast (h_filter.def_world.symm) ⟦y⟧);
+  convert h_filter.def_rel_forth $ Rxy;
+  simp_all;
+
+end
+
+
+
+section
+
+variable {M : Model} {T : FormulaSet ℕ} [T.SubformulaClosed]
+         (FM : Model) (filterOf : FilterOf FM M T)
+
+theorem filteration {x : M.World} {φ : Formula ℕ} (hs : φ ∈ T) : x ⊧ φ ↔ (cast (filterOf.def_world.symm) ⟦x⟧) ⊧ φ := by
+  induction φ using Formula.rec' generalizing x with
+  | hatom a =>
+    have := filterOf.def_valuation (cast filterOf.def_world.symm ⟦x⟧) a;
+    simp_all [Satisfies];
+  | hand φ ψ ihφ ihψ =>
+    constructor;
+    . rintro ⟨hφ, hψ⟩;
+      constructor;
+      . refine ihφ (FormulaSet.SubformulaClosed.mem_and₁ hs) |>.mp hφ;
+      . refine ihψ (FormulaSet.SubformulaClosed.mem_and₂ hs) |>.mp hψ;
+    . rintro ⟨hφ, hψ⟩;
+      constructor;
+      . refine ihφ (FormulaSet.SubformulaClosed.mem_and₁ hs) |>.mpr hφ;
+      . refine ihψ (FormulaSet.SubformulaClosed.mem_and₂ hs) |>.mpr hψ;
+  | hor φ ψ ihφ ihψ =>
+    constructor;
+    . rintro (hφ | hψ);
+      . left; exact ihφ (FormulaSet.SubformulaClosed.mem_or₁ hs) |>.mp hφ;
+      . right; exact ihψ (FormulaSet.SubformulaClosed.mem_or₂ hs) |>.mp hψ;
+    . rintro (hφ | hψ);
+      . left; exact ihφ (FormulaSet.SubformulaClosed.mem_or₁ hs) |>.mpr hφ;
+      . right; exact ihψ (FormulaSet.SubformulaClosed.mem_or₂ hs) |>.mpr hψ;
+  | himp φ ψ ihφ ihψ =>
+    constructor;
+    . rintro hφψ Qy RQxQy hφ;
+      obtain ⟨y, ey⟩ := Quotient.exists_rep (cast (filterOf.def_world) Qy);
+      apply (show Satisfies M y ψ → Satisfies FM Qy ψ by simpa [ey] using @ihψ y (FormulaSet.SubformulaClosed.mem_imp₂ hs) |>.mp)
+      have : ∀ φ ∈ T, Satisfies M x φ → Satisfies M y φ := by simpa [←ey] using filterOf.def_rel_back RQxQy;
+      apply this (φ ➝ ψ) hs hφψ;
+      . simp;
+      . apply ihφ (FormulaSet.SubformulaClosed.mem_imp₁ hs) |>.mpr;
+        convert hφ;
+        simp_all;
+    . rintro h y Rxy hφ;
+      apply ihψ (FormulaSet.SubformulaClosed.mem_imp₂ hs) |>.mpr;
+      apply h (filterOf.def_rel_forth Rxy);
+      apply ihφ (FormulaSet.SubformulaClosed.mem_imp₁ hs) |>.mp hφ;
+  | _ => trivial
+
+end
+
+abbrev standardFilterationValuation (Qx : FilterEqvQuotient M T) (a : ℕ) := (ha : (atom a) ∈ T) → Quotient.lift (λ x => M.Val x a) (by
+  intro x y h;
+  apply eq_iff_iff.mpr;
+  constructor;
+  . intro hx; exact h (.atom a) ha |>.mp hx;
+  . intro hy; exact h (.atom a) ha |>.mpr hy;
+) Qx
+
+
+abbrev coarsestFilterationFrame (M : Model) (T : FormulaSet ℕ) [T.SubformulaClosed] : Kripke.Frame where
+  World := FilterEqvQuotient M T
+  Rel Qx Qy :=
+    Quotient.lift₂ (λ x y => ∀ φ ∈ T, (x ⊧ φ → y ⊧ φ)) (by
+      intro x₁ y₁ x₂ y₂ hx hy;
+      apply eq_iff_iff.mpr;
+      constructor;
+      . intro h φ hφ hφ_x₂;
+        apply hy φ |>.mp;
+        apply h;
+        . exact hφ
+        . apply hx φ |>.mpr hφ_x₂;
+      . intro h φ hφ hφ_y₁;
+        apply hy φ |>.mpr;
+        apply h;
+        . exact hφ
+        . apply hx φ |>.mp hφ_y₁;
+    ) Qx Qy
+  rel_refl := by
+    intro Qx;
+    obtain ⟨x, rfl⟩ := Quotient.exists_rep Qx;
+    simp;
+  rel_trans := by
+    intro Qx Qy Qz RQxQy RQyQz;
+    obtain ⟨x, rfl⟩ := Quotient.exists_rep Qx;
+    obtain ⟨y, rfl⟩ := Quotient.exists_rep Qy;
+    obtain ⟨z, rfl⟩ := Quotient.exists_rep Qz;
+    simp_all;
+
+abbrev coarsestFilterationModel (M : Model) (T : FormulaSet ℕ) [T.SubformulaClosed] : Kripke.Model where
+  toFrame := coarsestFilterationFrame M T
+  Val := ⟨
+    standardFilterationValuation M T,
+    by
+      intro Qx Qy RQxQy a hQx ha;
+      obtain ⟨x, rfl⟩ := Quotient.exists_rep Qx;
+      obtain ⟨y, rfl⟩ := Quotient.exists_rep Qy;
+      apply RQxQy (.atom a) ha;
+      tauto;
+  ⟩
+
+instance coarsestFilterationModel.filterOf {M} {T : FormulaSet ℕ} [T.SubformulaClosed] : FilterOf (coarsestFilterationModel M T) M T where
+  def_valuation := by tauto
+  def_rel_forth := by
+    intro x y Rxy;
+    intro φ hφ;
+    apply Formula.Kripke.Satisfies.formula_hereditary Rxy;
+  def_rel_back := by tauto;
+
+
+-- TODO: might be wrong, because finest filteration is not transitive?
+/-
+abbrev finestFilterationFrame (M : Model) (T : FormulaSet ℕ) [T.SubformulaClosed] : Kripke.Frame where
+  World := FilterEqvQuotient M T
+  Rel Qx Qy := ∃ x y, Qx = ⟦x⟧ ∧ Qy = ⟦y⟧ ∧ x ≺ y
+  rel_refl := by
+    intro Qx;
+    obtain ⟨x, rfl⟩ := Quotient.exists_rep Qx;
+    use x, x;
+    simp;
+  rel_trans := by
+    rintro Qx Qy Qz ⟨x, y, ⟨rfl, rfl, Rxy⟩⟩ ⟨w, z, ⟨hyw, rfl, Ryz⟩⟩;
+    use x, z;
+    refine ⟨by tauto, by tauto, ?_⟩;
+    sorry;
+
+abbrev finestFilterationModel (M : Model) (T : FormulaSet ℕ) [T.SubformulaClosed] : Kripke.Model where
+  toFrame := coarsestFilterationFrame M T
+  Val := ⟨
+    standardFilterationValuation M T,
+    by
+      intro Qx Qy RQxQy a hQx ha;
+      obtain ⟨x, rfl⟩ := Quotient.exists_rep Qx;
+      obtain ⟨y, rfl⟩ := Quotient.exists_rep Qy;
+      apply RQxQy (.atom a) ha;
+      tauto;
+  ⟩
+
+instance finestFilterationModel.filterOf {M} {T : FormulaSet ℕ} [T.SubformulaClosed] : FilterOf (finestFilterationModel M T) M T where
+  def_valuation := by tauto
+  def_rel_back := by tauto;
+  def_rel_forth := by
+    intro x y Rxy;
+    intro φ hφ;
+    apply Formula.Kripke.Satisfies.formula_hereditary Rxy;
+-/
+
+end Kripke
+
+end LO.Propositional
